## L 

$\int\limits_{0}^{1} xe^{-x^2} dx$

$u = -x^2$

$du = -2x$

$-0.5\int\limits_{0}^{1} du e^{u}$

$-0.5\int\limits_{0}^{1} du e^{u}$

## J

$f(2) - f(-2) = 16$

$f'(x) = x^7 + k$

$f(x) = \frac{1}{8}x^8 + kx$

$f(x) = \frac{1}{8}x^8 + kx$

$\frac{1}{8}(2)^8 + 2k - (\frac{1}{8}(-2)^8 -2k) = 16$

$(-2)^8 = (2)^8$

$\frac{1}{8}(2)^8 + 2k - \frac{1}{8}(-2)^8 + 2k = 16$

$2k + 2k = 16$

$4k = 16$

$k = 4$

## A

$\int\limits_{0}^{1} x(x^2 + 2)^2 dx$

$u = x^2 + 2$
$du = 2x$

$0.5\int\limits_{0}^{1} du * u^2 dx$

$0.5\int\limits_{0}^{1} du * \frac{1}{3}u^3$

$0.5\int\limits_{0}^{1} 2x * \frac{1}{3}u^3$

$0.5\int\limits_{0}^{1} du * \frac{1}{3}u^3$

$\frac{1}{6}u^3 |_2^3$

$4.5 - 1.33$

$3.17$

## C

$\int \frac{3x^2}{\sqrt{x^3 + 1}}$

$u = x^3 + 1$
$du = 3x^2$

$2u^{0.5}$

## K

$24 - (-5)$