## Station 1
Find the derivative using two methods if $g(t) = \frac{t^2 - 1}{1 + t}$

$g(t) = \frac{t^2 - 1}{1 + t}$
$g(t) = \frac{(t - 1)(t + 1)}{1 + t}$
$g(t) = t - 1$
$g'(t) = 1$

$g'(t) = lim_{h->0}\frac{g(t + h) - g(t)}{h}$
$g'(t) = lim_{h->0}\frac{g(t + h) - t - 1}{h}$
$g'(t) = lim_{h->0}\frac{t + h - 1 - t - 1}{h}$
$g'(t) = lim_{h->0}\frac{h}{h}$
$g'(t) = lim_{h->0}1$
$g'(t) = 1$

**Go to Station 5**

## Station 5

Let $g(x) = x^{3/5}$. At what x-values, if any, is $g(x)$
a. Differentiable?
b. Continuous but not differentiable?
c. Neither continuous nor differentiable?

Continous at all points-- it's a polynomial. Therefore, `c` must be none. It must not be option `a`, since that would send us back to Station 1.  Ergo, option `b` must be correct, as it's the only one.

**Go to Station 2**

## Station 2

At what x-value is the slope of the function $f(x) = (2x^3 - 3x^2)/(6)$ equal to 6?

$f'(x) = \frac{6(6x^2 - 6x)}{36}$
$f'(x) = \frac{6x^2 - 6x}{6}$
$f'(x) = x^2 - x$

$6 = x^2 - x$
$6 = x^2 - x$
$0 = x^2 - x - 6$
$x = 3$ or  $x = -2$

**Go to Station 6**

## Station 6

$f(x) = \frac{cos(x)}{cos(x) - 2}$
$f'(x) = \frac{-sin(x)(cos(x) - 2) - cos(x)sin(x)}{(cos(x) - 2)^2}$
$f'(x) = 0 \impliedby x = n\pi$

**Go to Station 8**

## Station 8

Let $g(x)$ and and $g'(x)$ have  the following values
| x| g(x) | g'(x)|
| 0 | 9 | -2 |
| 1 | -3 | 4 |

$g(x)/(x^2+2)$
$(-2x^2 - 4 - 18)/(x^2+2)$
$(-2x^2 - 18x - 4)/(x^2+2)$
$(-2x^2 - 18x - 4)/(x^2+2)$
$(-2x^2 - 18x - 4)/(x^2+2)$
$-1$

**Go to Station 4**

## Station 4

Find the derivative using two methods if $f(x) = x^{-2} - 4x^{-3}$

$f'(x) = -2x^{-3} + 12x^{-4}$

$f'(x) = lim_{h->0} ( f(x+h) - f(x) )/h$
$f'(x) = lim_{h->0} ( f(x+h) - x^{-2} + 4x^{-3} )/h$
$f'(x) = lim_{h->0} ( f(x+h) - x^{-2} + 4x^{-3} )/h$
$f'(x) = lim_{h->0} ( (x+h)^{-2} - 4(x+h)^{-3} - x^{-2} + 4x^{-3} )/h$
$f'(x) = lim_{h->0} ( 1/(x^2 + 2xh + h^2) - 4/((x+h)^3) - x^{-2} + 4x^{-3} )/h$
$f'(x) = lim_{h->0} ( 1/(x^2 + 2xh + h^2) - 4/((x+h)(x^2 + 2xh + h^2)) - x^{-2} + 4x^{-3} )/h$
$f'(x) = lim_{h->0} ( 1/(x^2 + 2xh + h^2) - 4/(x^3 + x^2h + 4x^2h + 4xh^2 + h^3 + xh^2)) - x^{-2} + 4x^{-3} )/h$
$f'(x) = lim_{h->0} ( 1/(x^2 + 2xh + h^2) - 4/(x^3 + x^2h + 4x^2h + 4xh^2 + h^3 + xh^2)) - x^{-2} + 4x^{-3} )/h$
$f'(x) = -2x^{-3} + 12x^{-4}$

**Go to Station 7**

## Station 7

Write an equation for the line tangent to $h(x)$ at $x = 1$ if $h(X) = \frac{x}{e} + \frac{e}{x}$

$h'(x) = \frac{e}{e^2} + \frac{e}{x^2}$
$h'(x) = \frac{1}{e} + \frac{-e}{x^2}$
$h'(1) = \frac{1}{e} + \frac{-e}{1}$
$h'(1) = \frac{1}{e} - e$

$h(1) = 1/e + e/1$
$h(1) = 1/e + e$
$h(1) = 2e$

$y - 2e = (1/e - e)(x - 1)$

**Go to Station 3**

## Station 3
$f'(x) = 1 + xsin(x) + cos(x)$
$f''(x) = cos(x)$

