1) Use implicit differentiation to find the following for $y^2 - x^2 = 5$
	a) $\frac{dy}{dx}$ : $2y\frac{dy}{dx} - 2x = 0$
		$2y\frac{dy}{dx} = 2x$
		$\frac{dy}{dx} = \frac{2x}{2y}$
	b) $\frac{d^2y}{dx^2}$: 
2) Find $\frac{dy}{dx}$ if $e^y\cos(x) = x + 1$ and find an equation tangent to the graph at the point (0,0)
	$e^y\cos(x) = x + 1$
	$\frac{dy}{dx}e^y\cos(x) - \sin(x)e^y = 1$
	$\frac{dy}{dx}e^y\cos(x) = 1 + \sin(x)e^y$
	$\frac{dy}{dx}e^y = \frac{1 + \sin(x)e^y}{\cos(x)}$
	$\frac{dy}{dx} = \frac{1 + \sin(x)e^y}{e^y\cos(x)}$
	
	y = 0, x = 0
	$\frac{dy}{dx} = \frac{1 + \sin(0)e^0}{e^0\cos(0)}$
	$\frac{dy}{dx} = \frac{1 + \sin(0) * 1}{1 * 1}$
	$\frac{dy}{dx} = \frac{1 + \sin(0)}{1}$
	$\frac{dy}{dx} = 1 + \sin(0)$
	$\frac{dy}{dx} = 1$
	Tangent Line: $y=x$
	
	
3) Find $\frac{dy}{dx}$ at the point $(3, 8)$ for $5xy^\frac{2/3} - x^2y = -12$
	$\frac{10}{3}x\frac{1}{y^{1/3}}\frac{dy}{dx} + 5y^\frac{2}{3} - 2xy - x^2\frac{dy}{dx} = 0$
	$\frac{10}{3}3\frac{1}{8^{1/3}}\frac{dy}{dx} + 5*8^\frac{2}{3} - 2*3*8 - 3^2\frac{dy}{dx} = 0$
	$10\frac{1}{8^{1/3}}\frac{dy}{dx} + 5*8^\frac{2}{3} - 48 - 9\frac{dy}{dx} = 0$
	$10\frac{1}{2}\frac{dy}{dx} + 5*8^\frac{2}{3} - 48 - 9\frac{dy}{dx} = 0$
	$5\frac{dy}{dx} + 5*8^\frac{2}{3} - 48 - 9\frac{dy}{dx} = 0$
	$5\frac{dy}{dx} + 5*4 - 48 - 9\frac{dy}{dx} = 0$
	$5\frac{dy}{dx} + 20 - 48 - 9\frac{dy}{dx} = 0$
	$5\frac{dy}{dx} - 28 - 9\frac{dy}{dx} = 0$
	$5\frac{dy}{dx} - 9\frac{dy}{dx} = 28$
	$\frac{dy}{dx}(5 - 9) = 28$
	$\frac{dy}{dx} = \frac{28}{(5 - 9)}$
	$\frac{dy}{dx} = \frac{28}{5 - 9}$
	$\frac{dy}{dx} = \frac{-28}{4}$
	$\frac{dy}{dx} = -7$
	
	
	
	Find $\frac{dy}{dx}$ for $x^2y = 4$ 
	
	$2xy + \frac{dy}{dx}x^2 = 0$
	$\frac{dy}{dx}x^2 = -2xy$
	$\frac{dy}{dx} = \frac{-2xy}{x^2}$
	
	
	Find $\frac{d^2y}{dx^2}$
	
	$\frac{-2xy}{x^2}$
	
	$\frac{(-2y + -2\frac{dy}{dx}x) x^2 - -2y}{x^4} = \frac{6y}{x^3}$
	
	
	Is this relation decreasing at x=2?
	
	$2^2y = 4$
	$4y = 4$
	$y = 1$
	
	$\frac{-8}{4}$
	$-2$
	
The relation is decreasing at $(2,1)$ because $\frac{dy}{dx} < 0$

What is the concavity at (2,1)?

$\frac{6}{8}$
$\frac{3}{4}$

The relation is concave up at $(2,1)$ because $\frac{d^2y}{dx^2} > 0$ there.


$4\frac{2x-6}{3x^2-1}^3 + \frac{2(3x^2 - 1) - 6x(2x - 6)}{(3x^2 - 1)^2}$