## Part 1
1. $g(f(1)) = g(3) = 6$
2. $f(f(4)) = f(2) = 5$
3. $g(f(1)) = g(3) = 6$
4. $g'(f(4)^2) = g'(2^2) = g'(4) = 1$
5. $g'(f(4))^2 = g'(2)^2 = 4^2 = 16$

## Part 2
1. $f(x) = \sqrt{x}; f'(x) = \frac{1}{2\sqrt{x}}; g(x) = 3x^5 + 2x - 4; g'(x) = 15x^4 + 2$
2. $f(x) = x^6; f'(x) = 6x^5; g(x) = 3x - 1; g'(x) = 3$
3. $f(x) = \frac{1}{x}; f'(x) = -x^2; g(x) = 2x + 1; g'(x) = 2$
4. $f(x) = x^{2/3}; f'(x) = \frac{2}{3}x^{-1/3}; g(x) = 3 + 6\sqrt{x}; g'(x) = \frac{6}{2\sqrt{x}}$
5. $f(x) = \frac{4}{x^3}; f'(x) = \frac{-12}{x^4}; g(x) = 2x^2 - x - 1; g'(x) = 4x - 1$
6. $f(x) = x^5 = f'(x) = 5x^4; g(x) = 3 + sin(x); g'(x) = -cos(x)$
7. $f(x) = tan(x); f'(x)=sec(x)^2; g(x) = 3x; g'(x) = 3$
8. $f(x) = x^4; f'(x) = 4x^3; g(x) = cos(x); g'(x) = sin(x)$
9. $f(x) = e^x; f'(x) = e^x; g(x) = 5x - 2; g'(x) = 5$
10. $f(x) = ln(x); f'(x) = 1/x; g(x) = 3x^4 + x - 5; g'(x) = 12x^3 + 1$