1. $f(x) = x^2 + 5x + 1; c = -2$
  $f'(x) = lim_{h->0} (f(x+h)-f(x))/h$
  $f'(x) = lim_{h->0} ((x+h)^2 + 5(x+h) + 1 - x^2 + 5x + 1)/h$
  $f'(x) = lim_{h->0} ((x+h)^2 + 5x + 5h - x^2 - 5x)/h$
  $f'(x) = lim_{h->0} ((x+h)^2 + 5h - x^2)/h$
  $f'(x) = lim_{h->0} (x^2 + h^2 + 2xh + 5h - x^2)/h$
  $f'(x) = lim_{h->0} (h^2 + 2xh + 5h)/h$
 $f'(x) = lim_{h->0} h(h + 2x + 5)/h$
 $f'(x) = lim_{h->0} (h + 2x + 5)$
$f'(x) = lim_{h->0} (h + 2x + 5) = 2x + 5$
$f'(c) = -4 + 5 = 1$

2. $f(x) = x^3 - 4x^2 + x + 8; c = -2$
$f'(x) = lim_{h->0} (f(x+h)-f(x))/h$
$f'(x) = lim_{h->0} (((x+h)^3 - 4(x+h)^2 + (x+h) + 8)-(x^3 - 4x^2 + x + 8))/h$
$f'(x) = lim_{h->0} (((x+h)^3 - 4(x^2 + 2xh + h^2) + (x+h) + 8) + -x^3 + 4x^2 - x - 8)/h$
$f'(x) = lim_{h->0} (((x+h)^3 + -4x^2 + -8xh + -4h^2 + (x+h) + 8) + -x^3 + 4x^2 - x - 8)/h$
$f'(x) = lim_{h->0} (((x+h)^3 + -4x^2 + -8xh + -4h^2 + x + h + 8) + -x^3 + 4x^2 - x - 8)/h$
$f'(x) = lim_{h->0} (( (x+h)(x+h)(x+h) + -4x^2 + -8xh + -4h^2 + x + h + 8) + -x^3 + 4x^2 - x - 8)/h$
$f'(x) = lim_{h->0} (( (x+h)(x^2 + 2xh + h^2) + -4x^2 + -8xh + -4h^2 + x + h + 8) + -x^3 + 4x^2 - x - 8)/h$
$f'(x) = lim_{h->0} (( ((x+h)x^2 + (x+h)2xh + (x+h)h^2) + -4x^2 + -8xh + -4h^2 + x + h + 8 + -x^3 + 4x^2 - x - 8)/h$
$f'(x) = lim_{h->0} ((x^3+hx^2 + 2x^2h + 2xh^2 + xh^2 + h^2) + -4x^2 + -8xh + -4h^2 + x + h + 8 + -x^3 + 4x^2 - x - 8)/h$
$f'(x) = lim_{h->0} (x^3+hx^2 + 2x^2h + 2xh^2 + xh^2 + h^2 + -4x^2 + -8xh + -4h^2 + x + h + 8 + -x^3 + 4x^2 - x - 8)/h$
$f'(x) = lim_{h->0} (2x^2h + 2xh^2 + 2xh^2 + h^2 + -8xh + h)/h$
$f'(x) = lim_{h->0} h(2x^2 + 4xh + h + -8x + 1)/h$
$f'(x) = lim_{h->0} (2x^2 + 4xh + h + -8x + 1)$
$f'(x) = 2x^2 - 8x + 1$
$f'(c) = 2*4 + 16 + 1 = 25$

3. $f(x) = -0.7x + 2; c  = 3$
$f'(x) = lim_{h->0} (f(x+h)-f(x))/h$
$f'(x) = lim_{h->0} (-0.7(x+h) + 2 + 0.7x - 2)/h$
$f'(x) = lim_{h->0} (-0.7x - 0.7h + 2 + 0.7x - 2)/h$
$f'(x) = lim_{h->0} (-0.7x - 0.7h + 0.7x)/h$
$f'(x) = lim_{h->0} (-0.7h)/h$
$f'(x) = lim_{h->0} -0.7$
$f'(x) = -0.7$
$f'(c) = -0.7$

4. $f(x) = 1.3x - 3; c = 4$
$f'(x) = lim_{h->0} (f(x+h)-f(x))/h$
$f'(x) = lim_{h->0} (1.3(x+h) - 3 - 1.3x + 3)/h$
$f'(x) = lim_{h->0} (1.3x + 1.3h - 1.3x)/h$
$f'(x) = lim_{h->0} (1.3h)/h$
$f'(x) = lim_{h->0} 1.3$
$f'(x) = 1.3$
$f'(c) = 1.3$

5. $f(x) = 5; c = -1$
$f'(x) = lim_{h->0} (f(x+h)-f(x))/h$
$f'(x) = lim_{h->0} (5 - 5)/h$
$f'(x) = lim_{h->0} 0/h$
$f'(x) = 0$
$f'(c) = 0$

6. $f(x) = -2; c = 3$
$f'(x) = lim_{h->0} (f(x+h)-f(x))/h$
$f'(x) = lim_{h->0} (-2 + 2)/h$
$f'(x) = lim_{h->0} 0/h$
$f'(x) = 0$
$f'(c) = 0$

7. 
	1. I graphed the tangent line by using point-slope form; I used a slope of 2 bc of the derivative and a point of (1, 1) because that's the point.
	2. The line and the curve become more similar as I zoom in
	3. They are the same
	4. Because the graph is linear over a local range
	5. Because the local section is linear and the tangent line is equal to that line.
8. $g(x) = 5x^3$
$g'(x) = lim_{h->0} (g(x+h)-g(x))/h$
$g'(x) = lim_{h->0} (5(x+h)^3 - 5x^3)/h$
$g'(x) = lim_{h->0} (5(x^2 + xh +h^2)(x+h) - 5x^3)/h$
$g'(x) = lim_{h->0} (5(hx^2 + x^3 + x^2h + xh^2 + xh^2 + h^3) - 5x^3)/h$
$g'(x) = lim_{h->0} (5hx^2 + 5x^3 + 5x^2h + 5xh^2 + 5xh^2 + 5h^3 - 5x^3)/h$
$g'(x) = lim_{h->0} (5hx^2 + 5x^2h + 5xh^2 + 5xh^2 + 5h^3)/h$
$g'(x) = lim_{h->0} h(5x^2 + 5x^2 + 5xh + 5xh + 5h^2)/h$
$g'(x) = lim_{h->0} (5x^2 + 5x^2 + 5xh + 5xh + 5h^2)$
$g'(x) = lim_{h->0} 10x^2 + 10xh + 5h^2$
$g'(x) = 10x^2$
9. $v(t) = 10t^2 - 5t + 7$
$v'(x) = lim_{h->0} (v(x+h)-v(x))/h$
$v'(x) = lim_{h->0} (v(x+h) - 10t^2 + 5t - 7)/h$
$v'(x) = lim_{h->0} (10(t+h)^2 - 5t + 5h + 7 - 10t^2 + 5t - 7)/h$
$v'(x) = lim_{h->0} (10(t+h)^2 - 5h - 10t^2)/h$
$v'(x) = lim_{h->0} (10(t^2 + th + h^2) - 5h - 10t^2)/h$
$v'(x) = lim_{h->0} (10t^2 + 10th + 10h^2 - 5h - 10t^2)/h$
$v'(x) = lim_{h->0} (10th + 10h^2 - 5h)/h$
$v'(x) = lim_{h->0} h(10t + 10h - 5)/h$
$v'(x) = (10t - 5)$
10. 
	1. 
        $h(x) = -5x^2 + 20x$
		$h'(x) = lim_{h->0} (h(x+h)-h(x))/h$
		$h'(x) = lim_{h->0} (-5(x+h)^2 + 20(x+h) + 5x^2 - 10x)/h$
		$h'(x) = lim_{h->0} (-5(x^2 + h^2 + xh) + 20(x+h) + 5x^2 - 20x)/h$
		$h'(x) = lim_{h->0} (-5x^2 - 5h^2 - 5xh + 20x + 20h + 5x^2 - 20x)/h$
		$h'(x) = lim_{h->0} (-5h^2 - 5xh + 20h)/h$
		$h'(x) = lim_{h->0} h(-5h - 5x + 20)/h$
		$h'(x) = lim_{h->0} -5h - 5x + 20$
		$h'(x) = -5x + 20$
	2. $h'(3) = 5$ It was going up because $5 > 0$.
	3. It was above where Chuck threw it, because $h(3) = 15$ and $15 > 0$
	4. It was at its highest point at $x=4$ because that is the peak of the parabola.
11. $h'(x) = lim_{h->0} (h(x+h)-h(x))/h$
	$h'(x) = lim_{h->0} (0.6x^2 + 0.6xh + 0.6h^2 - 0.6x^2)/h$
	$h'(x) = lim_{h->0} (+ 0.6xh + 0.6h^2)/h$
	$h'(x) = lim_{h->0} h(0.6x + 0.6h)/h$
	$h'(x) = lim_{h->0} (0.6x + 0.6h)$
	$h'(x) = lim_{h->0} 0.6x + 0.6h$
	$h'(x) = 0.6x$
	$y = 1.8(x + 3) - 5.4$
12. 
	1. $f'(x) = lim_{h->0} (f(x+h)-f(x))/h$
		$f'(x) = lim_{h->0} (\sqrt{x+h}-\sqrt{x})/h$
		$f'(x) = lim_{h->0} (\sqrt{x+h}-\sqrt{x})/h$
		$f'(x) = lim_{h->0} (\sqrt{x+h}-\sqrt{x})/h$
		$f'(x) = lim_{h->0} (\sqrt{x+h}-\sqrt{x})(\sqrt{x+h}+\sqrt{x})/h(\sqrt{x+h}+\sqrt{x})$
		$f'(x) = lim_{h->0} ((x + h) - x) / h(\sqrt{x+h}+\sqrt{x})$
		$f'(x) = lim_{h->0} h / h(\sqrt{x+h}+\sqrt{x})$
		$f'(x) = \frac{1}{\sqrt{x}+\sqrt{x}}$
		$f'(x) = \frac{1}{2\sqrt{x}}$
	2. $f'(x) = lim_{h->0} (f(x+h)-f(x))/h$
		$f'(x) = lim_{h->0} (1/(x+h)- 1/x)/h$
		$f'(x) = lim_{h->0} (x/x(x+h)- (x+h)/x(x+h))/h$
		$f'(x) = lim_{h->0} ((x - (x+h))/x(x+h))/h$
		$f'(x) = lim_{h->0} ((x - x + h))/x(x+h))/h$
		$f'(x) = lim_{h->0} (h)/x(x+h))/h$
		$f'(x) = lim_{h->0} 1/(x(x+h))$
		$f'(x) = lim_{h->0} 1/(x^2)$
		$f'(x) = 1/(x^2)$
		$f'(x) = \frac{1}{x^2}$