1. 
  a. $f(x) = (3x^2 + x)(e^x)$
     $f'(x) = (6x + 1)(e^x) + (3x^2 + x)(e^x)$
   b. $y = \frac{e^x}{4+x^2}$
       $y' = \frac{e^x(4+x^2) - e^x(2x)}{(4+x^2)^2}$
2. $f(x) = (3x - 1)(e^x)$ 
     $f'(x) = 3e^x + e^x(3x -1)$
    $f'(x) = 3e^x + 3xe^x - e^x$
    $f'(x) = 3xe^x + 2e^x$
   $f'(x) = e^x(3x + 2)$
   $e^x > 0$, so for $f'(x) < 0$, $3x + 2 < 0$

	$f'(x) = 0$ when $3x + 2 = 0$, so $f'(\frac{-2}{3}) = 0$
	$f'(x) < 0, x<\frac{-2}{3}$
	$f'(x) > 0, x>\frac{-2}{3}$
3. 
    a.  $h(x) = 5f(x) + 2g(x)$
		$h'(2) = -10 + 8$
		$h'(2) = -2$
	b. $h(x) = f(x) * g(x)$
	    $h'(x) = f(x)g'(x) + g(x)f'(x)$
		$h'(2) = 3*4 + 2*-2$
		$h'(2) = 12 - 4$
		$h'(2) = 8$
	c. $h(x) = f(x)/g(x)$
	$h'(x) = (f'(x)g(x) - f(x)g'(x))/g(x)^2$
	$h'(2) = (-2*2 - 3*4)/4$
	$h'(2) = (-4 - 12)/4$
	$h'(2) = -4$
	d. $h(x) = g(x)/(1+f(x))$
		$h'(x) = (f'(x)g(x) - (1+f(x))*g'(x) )/(1+f(x))^2$
		$h'(x) = (-2 * 2 - (1+3)*4 )/(1+3)^2$
		$h'(x) = (-2 * 2 - 16 )/16$
		$h'(x) = (-4 - 16 )/16$
		$h'(x) = -5/4$
		$h'(x) = -1.2$
4. $y' = 2 + \frac{ e^x(x^2+1) - e^x(2x) }{(x^2 + 1)^2}$
	$y'(3) = 2 + \frac{ e^3(10) - e^3(6) }{100}$
	$y'(3) = 2 + \frac{ 10e^3 - 6e^3 }{100}$
	$y'(3) = 2 + \frac{ 4e^3}{100}$
	$y'(3) = 2 + 0.04e^3$
	$y'(3) = 2 + 0.04e^3$
	 $y(3) = 9 + 0.1e^3$
	 $t_y = (2 + 0.04e^3)(x - 3) + 9 + 0.1e^3$
	 $t_y = 2x - 6 + 0.04e^3(x - 3) + 9 + 0.1e^3$
	 $t_y = 2x + 0.04e^3x - 0.12e^3 + 3 + 0.1e^3$
	 $t_y = 2x + 0.04e^3x + 3 - 0.02e^3$
	 $t_y = 2x + 0.04e^3x - 0.02e^3 + 3$
	 
	 5.  
		a. $f(x) = 2x^5 - 6x^2$
			$f'(x) = 10x^4 - 12x$
		b. $f'(x) = 3*2x^2 + 4x(x^3 - 3)$
		
6. $g(t) = e^t\frac{1}{t^2}$
	$g'(t) = e^t\frac{1}{t^2} + e^t\frac{2}{-x^3}$
7. 
	a. $h(x) = -2x^5 * f(x)$
		$f(4.5) = -1$
		$f'(4.5) = 2$
		$h'(4.5) = -1*-10x^4 + 2*-2x^5$
		$h'(4.5) = 10x^4 - 4x^5$
		$h'(4.5) = 10x^4 - 4x^5$
		$h'(4.5) = -4x^5 + 10x^4$
		$h'(4.5) = âˆ’3280.5$
		
	b. $k(x) = \frac{3f(x)}{x^2}$
		$k'(x) = \frac{3f'(x) * x^2 - 3f(x) * 2x}{x^4}$
		$f(3) = -1$
		$f'(3) = -1$
		$k'(3) = \frac{3*-1*x^2 - 3*-1*2x}{x^4}$
		$k'(3) = \frac{-3x^2 - -6x}{x^4}$
		$k'(3) = \frac{-3x - -6}{x^3}$
		$k'(3) = \frac{-3x + 6}{x^3}$
		$k'(3) = \frac{-9 + 6}{27}$
		$k'(3) = \frac{3}{27}$
		$k'(3) = \frac{1}{9}$
	