# The Chain Rule

$$
h(x) = f(g(x)) \implies h'(x) = f'(g(x)) * g'(x)
$$


$h(x) = (x^2 + 3)^4$
$h'(x) = 4(x^2 + 3)^3 * 2x$
$h'(x) = 4(x^2 + 3)^3 * 2x$
$h'(x) = 4(x^2 + 3)^3 * 2x$

$h(x) = \sqrt{3x^5 + 2x - 4}$
$h(x) = 3x^5 + 2x - 4^{1/2}$
$h(x) = (3x^5 + 2x - 4)^{1/2}$
$h'(x) = 0.5(3x^5 + 2x - 4)^{-1/2} * (15x^4 + 2)$
$h'(x) = 0.5(3x^5 + 2x - 4)^{-1/2} * (15x^4 + 2)$


$h(x) = sin(3x)$
$h'(x) = cos(3x) * 3$
$h'(x) = 3cos(3x)$

$h(x) = e^{x^2+1}$
$h(x) = e^{x^2+1} * 2x$


$h(x) = \frac{sin(x)^2}{tan(x)}$
$h(x) = sin(x)^2 * cos(x)/sin(x)$
$h(x) = sin(x) * cos(x)$
$h'(x) = -sin(x)^2 + cos(x)^2$
$h'(\pi/3) = -sin(\pi/3)^2 + cos(\pi/3)^2$
$h'(\pi/3) = -(\sqrt{3}/2)^2 + (1/2)^2$
$h'(\pi/3) = -3/4 + 1/4$
$h'(\pi/3) = -1/2$

$h(x) = sin(x) * cos(x)$
$h(\pi/3) = \sqrt{3}/2 * 1/2$
$h(\pi/3) = \sqrt{3}/4$

$y = -0.5(x - \pi/3) + \sqrt{3}/4$
