## Part I

1. $\pi\int_{-1}^2 ((x + 3)^2 - (x^2 + 1)^2) dx = 23.4\pi$
2. $\pi\int_{-0.25\pi}^{0.25\pi} (2 - \sec{x}^2) dx 1.505\pi$
3. $\pi\int_0^8 (2^2 - \sqrt[3]{y}^2) dy = 12.8\pi$


## Part II

1.  
	R = $2x$
	r = *n/a*
	$V = \pi\int_0^3 ((2x)^2) dx = 36\pi$
2. 
	R = $3$
	r = $0.5y$
	$V = \pi\int_0^6 (3^2 - (0.5y)^2) dy = 36\pi$
3. 
	R = $1 + \sqrt{x}$
	r = $1$
	$V = \pi\int_0^4 ((1 + \sqrt{x})^2 - (1)^2) dx = 18\frac{2}{3}\pi$
4.  
	R = $4$
	r = $(y - 1)^2$
	$V = \pi\int_1^3 (4^2 - ((y-1)^2)^2) dy = 25.6\pi$
5. 
	R = $e^x$
	r = *n/a*
	$V = \pi\int_0^1 ((e^x)^2) dx = 3.195\pi$
6. R = $1$
	r = $\ln(y)$
	$V = \pi \int_0^e (1^2 - \ln(y)^2) dy = 2\pi$

	