1. $s^2$
	$\int_0^3 (1 - \frac{x}{3})^2 dx$
	$\int_0^3 (\frac{1}{9}x^2 -\frac{2}{3}x + 1) dx$
	$(\frac{1}{9*3}x^3 -\frac{1}{3}x^2 + x) |_0^3$
	$\frac{1}{9*3}(3)^3 -\frac{1}{3}(3)^2 + 3$
	$1 -3 + 3$
	$1$
2. $\int_{0}^{3} (5(2-\frac{2}{3}x)^2) dx$
	$20$
3. $x^2$
	$\int_0^1 0.5(\pi(0.5x^2)^2) dx$
	$\int_0^1 0.5 * \pi * (0.5x^2)^2 dx$
	$\pi * \int_0^1 0.5(0.5x^2)^2 dx$
	$\frac{\pi}{40}$
4. $\frac{\sqrt{3}}{2}s$
	$0.5\frac{\sqrt{3}}{2}ss$
	$\frac{\sqrt{3}}{4}s^2$
	$\int_0^2 (\frac{\sqrt{3}}{4}(x^3)^2) dx$
	$\int_0^2 (\frac{\sqrt{3}}{4} x^6) dx$
	$\frac{\sqrt{3}}{4 * 7} x^7 |_0^2$
	$\frac{\sqrt{3}}{4 * 7} x^7 |_0^2$
	$\frac{\sqrt{3}}{4 * 7} (2)^7$
	$\frac{\sqrt{3}}{7} (32)$
5. $(x-2)^2 - 4\cos(\frac{\pi x}{4})$
	$0.5ss$
	$0.5s^2$
	$0.5((x-2)^2 - 4\cos(\frac{\pi x}{4}))^2$
	$\int_0^2 (0.5((x-2)^2 - 4\cos(\frac{\pi x}{4}))^2) dx$
	$1.775$
6. $x = (y + 1)^2$
	$\pi \int_0^1 ((y + 1)^2)^2 dy$
	$\pi \int_0^1 (y + 1)^4 dy$
	$\pi \int_0^1 (y + 1)^4 dy$
	$\pi ( \frac{1}{5}(y + 1)^5|_0^1 )$
	$\pi ( \frac{1}{5}(1 + 1)^5 )$
	$\pi ( \frac{1}{5}(2)^5 )$
	$\pi ( \frac{1}{5}32 )$
	$\frac{31}{5}\pi$
---
8. $y = 4x$ $y = 8$
	$R = 8 - 4x$
	$R = 8 - 4x$
	$\pi\int_0^2 ((8 - 4x)^2) dx$
	$8\pi$
9. $x = \arcsin(y)$
	$R = (1 - \arcsin(y))$
	$\pi\int_0^{\sin(1)} (1 - \arcsin(y))^2 dy$
10. $R = 3 - 2x^2$ $r = 3 - 2x$
	$\pi \int_0^1 ((3 - 2x^2)^2 - (3 - 2x)^2) dx$
11. $R = 0.5\pi y + 3$ $r = \arcsin(y) + 3$
	$\pi \int_0^1 ((0.5\pi y + 3)^2 - (\arcsin(y) + 3)^2 ) dy$
---
13. $x = y^2 + 2$
	$\pi\int_{0}^{3} (( 11-(y^2+2) )^2) dy$
14. $R = 3 - (x^2 - 1)$ $r = 3 - (1 - x^2)$
	$\pi \int_{-1}^1 ((3 - (x^2 - 1))^2 - (3 - (1 - x^2))^2) dx$
	$\pi \int_{-1}^1 ((3 - x^2 + 1)^2 - (3 - 1 + x^2)^2) dx$
	$\pi \int_{-1}^1 ((4 - x^2)^2 - (2 + x^2)^2) dx$
	$\pi \int_{-1}^1 (x^4 -8x^2 + 16 - (x^4 + 4x^2 + 4)) dx$
	$\pi \int_{-1}^1 (x^4 -8x^2 + 16 - x^4 - 4x^2 - 4) dx$
	$\pi \int_{-1}^1 (x^4 -12x^2 + 12) dx$
	$\pi ((0.2x^5 -4x^3 + 12x) |_{-1}^1)$
	$\pi ((0.2x^5 -4x^3 + 12x) |_{-1}^1)$