1. 
	a. $5x^2 = -4y^3 - 3y^2 + 2$
		$10x = -12y^2\frac{dy}{dx} - 6y\frac{dy}{dx} + 0$
		$10x = -12y^2\frac{dy}{dx} - 6y\frac{dy}{dx}$
		$\frac{10x}{} = \frac{dy}{dx}(-12y^2 - 6y)$
		$\frac{10x}{-12y^2 - 6y} = \frac{dy}{dx}$
	b. $2x^3 + 3y^2 + 4x = 5$
		$6x^2 + 6y\frac{dy}{dx} + 4 = 0$
		$\frac{dy}{dx} = \frac{-6x^2 - 4}{6y}$
	c. $sin(y) + 3 = y + cos(x)$
		$cos(y)\frac{dy}{dx} = \frac{dy}{dx} - sin(x)$
		$cos(y)\frac{dy}{dx} - \frac{dy}{dx} = -sin(x)$
		$\frac{dy}{dx}(cos(y) - 1) = -sin(x)$
		$\frac{dy}{dx} = \frac{-sin(x)}{cos(y) - 1}$
	d. $cos(y^3) = x^3 + 2x + 5$
		$-sin(y^3)3y^2\frac{dy}{dx} = 3x^2 + 2$
		$\frac{dy}{dx} = \frac{3x^2 + 2}{-sin(y^3)3y^2}$

2. Find the points which have a vertical tangent line
	a. $4x^2 + y^2 - 8x + 4y + 4 = 0$
		$8x + 2y\frac{dy}{dx} - 8 + 4\frac{dy}{dx} = 0$
		$2y\frac{dy}{dx} + 4\frac{dy}{dx} = -8x + 8$
		$\frac{dy}{dx}(2y + 4) = -8x + 8$
		$\frac{dy}{dx} = \frac{-8x + 8}{2y + 4}$
		$2y + 4 = 0; -8x + 8 \not= 0$
		$y = -2$
		$4x^2 + (-2)^2 - 8x + 4*-2 + 4 = 0$
		$4x^2 + 4 - 8x - 8 + 4 = 0$
		$4x^2 - 8x = 0$
		$4(x^2 - 2x) = 0$
		$4x(x - 2)= 0$
		$\{(0, -2), (2, -2)\}$
	b. $x^2 + xy + y^2 = 6$
		$2x + x\frac{dy}{dx} + y + 2y\frac{dy}{dx} = 0$
		$x\frac{dy}{dx} + 2y\frac{dy}{dx} = 2x - y$
		$\frac{dy}{dx}(x - 2y) = 2x - y$
		$\frac{dy}{dx} = \frac{2x - y}{x - 2y}$
		$x - 2y = 0$
		$x = 2y$
		
		$(2y)^2 + 2yy + y^2 = 6$
		$4y^2 + 2y^2 + y^2 = 6$
		$7y^2 = 6$
		$y^2 = \frac{6}{7}$
		$y = \pm\sqrt{\frac{6}{7}}$
		
		$x^2 + x(\pm\sqrt{\frac{6}{7}}) + \frac{6}{7} = 6$
		$x^2 + x(\pm\sqrt{\frac{6}{7}}) + \frac{6}{7} - \frac{42}{7} = 0$
		$x^2 + x(\pm\sqrt{\frac{6}{7}}) - \frac{36}{7} = 0$
		$x^2 + x\sqrt{\frac{6}{7}} - \frac{36}{7} = 0$
		$x^2 + x\sqrt{\frac{6}{7}} - \frac{36}{7} = 0$
		quadratic formula time!
		$\frac{-\sqrt{\frac{6}{7}} \pm \sqrt{\frac{6}{7} - \frac{144}{7}}}{2}$
		$\frac{-\sqrt{\frac{6}{7}} \pm \sqrt{\frac{-138}{7}}}{2}$
		$\frac{-\frac{\sqrt{6}}{\sqrt{7}} \pm \frac{\sqrt{-138}}{\sqrt{7}}}{2}$
		$\frac{-\frac{\sqrt{6} \pm \sqrt{138}}{\sqrt{7}}}{2}$
		$-\frac{\sqrt{6} \pm \sqrt{138}}{2\sqrt{7}}$
		$-\frac{\sqrt{6} \pm \sqrt{23}\sqrt{6}}{2\sqrt{7}}$
		$-\frac{-\sqrt{22}\sqrt{6} or \sqrt{24}\sqrt{6}}{2\sqrt{7}}$
		$-\frac{2(-\sqrt{11}\sqrt{6} or \sqrt{12}\sqrt{6})}{2\sqrt{7}}$
		$-\frac{-\sqrt{11}\sqrt{6} or \sqrt{12}\sqrt{6}}{\sqrt{7}}$
		$-\frac{-\sqrt{11}\sqrt{6} or \sqrt{12}\sqrt{6}}{\sqrt{7}}$
		$\frac{\sqrt{11}\sqrt{6}}{\sqrt{7}} or \frac{-\sqrt{12}\sqrt{6}}{\sqrt{7}}$
		
		$\{(\frac{\sqrt{11}\sqrt{6}}{\sqrt{7}}, \sqrt{\frac{6}{7}}), (\frac{-\sqrt{12}\sqrt{6}}{\sqrt{7}}, \sqrt{\frac{6}{7}})\}$		
3. Find derivatives
	a. $y = \arcsin(4x)$
		$y' = \frac{1}{\sqrt{1- (4x)^2}} * 4$
		$y' = \frac{1}{\sqrt{1- 16x^2}} * 4$
		$y' = \frac{4}{\sqrt{1- 16x^2}}$
	b. $y = \arccos(10x)$
		$y' = -\frac{1}{\sqrt{1- (10x)^2}} * 10$
		$y' = -\frac{1}{\sqrt{1- 100x^2}} * 10$
		$y' = \frac{-10}{\sqrt{1 - 100x^2}}$
	c. $y = \arctan(\ln(x))$
		$y' = \frac{1}{1 + ln(x)^2} * \frac{1}{x}$
		$y' = \frac{1}{x + xln(x)^2}$
	d. $y = sec^{-1}(\frac{x}{3})$
		$y' = \frac{1}{|\frac{x}{3}| \sqrt{x^2 - 1}} * \frac{1}{3}$
		$y' = \frac{1}{3|\frac{x}{3}| \sqrt{x^2 - 1}}$
		$y' = \frac{1}{|x| \sqrt{x^2 - 1}}$