$$(f^{-1})' = \frac{1}{f'(f^{-1}(x))}$$

1.
	a. $f^{-1} = \root {3} \of {-0.5x + 2.5}$
		$(f^{-1})'(x) = \frac{1}{\root {3} \of {-0.5(6x^2) + 2.5}}$
		$(f^{-1})'(x) = \frac{1}{\root {3} \of {-3x^2 + 2.5}}$
		$(f^{-1})'(7) = \frac{1}{\root {3} \of {-3 * 49 + 2.5}}$
		$(f^{-1})'(7) = \frac{1}{\root {3} \of {-147 + 2.5}}$
		$(f^{-1})'(7) = \frac{1}{\root {3} \of {-144.5}}$
		$(f^{-1})'(7) = \frac{1}{\root {3} \of {-144.5}}$
		$(f^{-1})'(7) = \frac{1}{-5.24754231}$
		$(f^{-1})'(7) = -0.1905654$
		
  b. unit circle! $\frac{\pi}{6}$



3. $c$