- Sometimes, we take a derivative of a fun ction.
- Sometimes, you have to takea derivative of a **relation**-- an equation that that *isn't* a function (e.g. $y^2 + x^2 = 25$)
- In an implicit relationship, it is **implied** that $y$ is a function of $x$

## How 

Find the derivative of each term **with respect to x**. That means when you try to take the derivitive of something with $y$, just multiply it by $\frac{dy}{dx}$ (or $y'$, but don't do that yet)

$x^2 + y^2 = 25$
$2x + 2y * \frac{dy}{dx} = 0$ 
$2y * \frac{dy}{dx} = -2x$ 
$\frac{dy}{dx} = -x/y$


## Practice

a. $\frac{d}{dx}[y^3] = 3y^2 * \frac{dy}{dx}$

c. $\frac{d}{dx}[xy] = 1y + x * 1 * \frac{dy}{dx}$

e. $\frac{d}{dx}[x^2y^4] = 2xy^4 * 4x^2\frac{dy}{dx}y^3$


## Practice Two

2. $y = sin(x) + cos(y)$
	$\frac{dy}{dx} = cos(x)$
	$sin(y)\frac{dy}{dx} + \frac{dy}{dx} = cos(x)$
	$\frac{dy}{dx}(sin(y) =+ 1) = cos(x)$
	$\frac{dy}{dx} = \frac{cos(x)}{sin(y) + 1}$
	
3. $x^3 + x^2y + 4y^2 = 6$
	$3x^2 + x^2 + 2y * \frac{dy}{dx} + 8y * \frac{dy}{dx} = 0$
	$3x^2 + x^2 * \frac{dy}{dx} + 2xy + 8y * \frac{dy}{dx} = 0$
	$3x^2 + 2xy = - x^2\frac{dy}{dx} - 8y\frac{dy}{dx}$
	$3x^2 + 2xy = \frac{dy}{dx}(-x^2 - 8y)$
	$3x^2 + 2xy = \frac{dy}{dx}(-x^2 - 8y)$
	$-\frac{3x^2 + 2xy}{x^2 + 8y} = \frac{dy}{dx}$
	$\frac{dy}{dx} = -\frac{3x^2 + 2xy}{x^2 + 8y}$
	
	
	4. Find the equation of the line tangent to the graph of the given relation at the point $(-2, 3)$
		$x(xy + y^2) = 3x$
		$(xy + y^2) = 3$
		$xy + y^2 = 3$
		$x * \frac{dy}{dx} + yx + 2y \frac{dy}{dx} = 3$
		$x * \frac{dy}{dx} + 2y \frac{dy}{dx} = 3 - yx$
		$\frac{dy}{dx}(x + 2y) = 3 - yx$
		this was wrong because you can't factor out at the start or it'll give wrong answers$\frac{dy}{dx} = \frac{3 - yx}{x+2y}$~~	
		
		$\frac{dy}{dx} (-2,3) = \frac{3 - 2(-2)(3) - 9}{4 -12}$
		$\frac{dy}{dx} (-2,3) = \frac{3 + 12 - 9}{4 -12}$
		$\frac{dy}{dx} (-2,3) = \frac{3 + 3}{-8}$
		$\frac{dy}{dx} (-2,3) = \frac{6}{-8}$
		$\frac{dy}{dx} (-2,3) = \frac{-3}{4}$
		$\frac{dy}{dx} (-2,3) = \frac{-3}{4}$