1. $h(x) = x^2 - x + 2$
$h'(x) = lim_{h->0} (f(x + h) - f(x)) / (h)$
$h'(x) = lim_{h->0} (f(x + h) - x^2 - x + 2) / (h)$
$h'(x) = lim_{h->0} ((x + h)^2 - x - h + 2 - x^2 + x - 2) / (h)$
$h'(x) = lim_{h->0} ((x + h)^2 - h - x^2) / (h)$
$h'(x) = lim_{h->0} (x^2 + 2xh + h^2 - h - x^2) / (h)$
$h'(x) = lim_{h->0} (2xh + h^2 - h) / (h)$
$h'(x) = lim_{h->0} h(2x + h - 1) / (h)$
$h'(x) = lim_{h->0} (2x + h - 1)$
$h'(x) = 2x - 1$
2. $f(x) = x^2 - 1$
    $f'(2) = lim_{x->a} (f(x) - f(a)) / (x-a)$
	$f'(2) = lim_{x->a} (x^2 - 1 - a^2 + 1) / (x-a)$
	$f'(2) = lim_{x->a} (x^2 - a^2) / (x-a)$
	$f'(2) = lim_{x->a} (x-a)(x+a) / (x-a)$
	$f'(2) = lim_{x->a} (x+a)$
	$f'(2) = 2x$
	$f'(2) = 4$