ex1) $y = \arcsin(x)$

**Step 1:** Rewrite the equation without the inverse:
$sin(y) = x$

**Step 2** Draw and label a right triangle and label it. Label all the sides using the Pythagorean method. Use SOHCAHTOA.

**Step 3** Find the implicit derivative of the rewritten equation:

$cos(y)\frac{dy}{dx} = 1$
$\frac{dy}{dx} = \frac{1}{cos(y)}$

**Step 4** 
Use the triangle to rewrite the implicit derivative in terms of x. This will solve for y.

$\frac{dy}{dx} = \frac{1}{\sqrt{1-x^2}} = (1-x^2)^{-0.5}$


ex2) $y = \arccos(x)$

$x = cos(y)$

\*triangle\*
   
$\frac{dy}{dx} = \frac{1}{-x^2 * -sin(y)}$


ex4) 
$y= cot^{-1}(x)$
$x = cot(y)$

$x = cot(y)$
$1 = csc(y)^2\frac{dy}{dx}$
$\frac{1}{csc(y)^2} = \frac{dy}{dx}$

```   y
    x
        
  1
```

$\frac{1}{csc(y)^2} = \frac{dy}{dx}$

$\frac{dy}{dx} = \frac{1}{csc(y^2)}$
$\frac{dy}{dx} = \frac{1}{csc(y^2)}$


ex5) $sec(y) = x$

$sec(y)tan(y)\frac{dy}{dx} = 1$
$\frac{dy}{dx} = \frac{1}{sec(y)tan(y)}$

**When x is on the triangle's hypotenuse, take the ABSOLUTE VALUE in your answer**

ex6) $csc(y) = x$

$-csc(y)cot(y)\frac{dy}{dx} = 1$
$\frac{dy}{dx} = \frac{1}{-csc(y)cot(y)}$

```
     y



    /       |
   /        |
  x         1
 /          |
/sqrt(x^2-1)|

```



**Practice**

$y=\arcsin(3x)$

$y=arcsin'(3x) * 3$


$sin(y) = 3x$
$\frac{dy}{dx} = \frac{3}{cos(y)}$
$\frac{dy}{dx} = \frac{3}{\sqrt{1 - 9x^2}}$


*Alternative Method: Chain Rule*

If you can remember all 6 derivatives of inverse functions, you can simply chain-rule it in.


2. $y=\arctan(4x^2)$
$y=\arctan(4x^2)$

$x = tan(y)$
```
            y



    /        |
   /         |
  /          1
 sqrt(x^2+1) |
/_____x______|

```

$\frac{dy}{dx} = \frac{1}{sec(y)^2}$

$\frac{dy}{dx} = \frac{1}{sec(y)^2}$



Write the eqation of the line tangent to the function $y = \arcsin(x)$ at $x = \frac{\sqrt{3}}{2}$

oh this is easy. which angle's sine is $\frac{\sqrt{3}}{2}$? $\frac{\pi}{3}$!

$y - \frac{\pi}{3} = \frac{1}{\sqrt{0.25}}(x - \frac{sqrt{3}}{2})$


