1. $\int 0.25x^2 dx = \frac{0.25x^3}{3} + c$
2. $y = \cos(x) y'(x) = -\sin(x) -\sin(0.5\pi) = -1$
3. $2((\sin(\sqrt{x}))^2)$ $4(\sin(\sqrt{x})) * \cos(\sqrt{x}) * \frac{1}{\sqrt{x}}$ ==COME BACK TO==
---
5. $f''(x) = 24x - 12x^2 = x(24 - 12x) = 12x(2 - x) = -12x(x - 2)$
	$f''(1) > 0$
	$f''(-1) < 0$
	$f''(3) < 0$
6. $1 + \frac{dy}{dx}y^{-2/3} = \frac{dy}{dx}$
   $1 = \frac{dy}{dx} - \frac{dy}{dx}y^{-2/3}$
   $1 = \frac{dy}{dx}(1 - y^{-2/3})$
   $\frac{1}{(1 - y^{-2/3})} = \frac{dy}{dx}$
   $\frac{1}{(1 - 8^{-2/3})} = \frac{1}{(1 - \frac{1}{8^{2/3}})} = \frac{1}{(1 - \frac{1}{(64)^{1/3}})} = \frac{1}{(1 - \frac{1}{4})} = \frac{1}{\frac{3}{4}}= \frac{4}{3}$
7. $5x^4 - \ln(5)5^x$
---
9. $e^{\inf} > \inf^2$
10. $y = 2x; y = 4x - x^2$
	$2x = x(4 - x) \implies (x = 0 \lor x = 2)$
	$\int_0^2 ((4x - x^2) - (2x)) dx = \int_0^2 (4x - x^2 - 2x) dx = \int_0^2 (2x - x^2) dx = (x^2 - \frac{1}{3}x^3)|_0^2 = (2^2 - \frac{1}{3}(2)^3) = (4 - \frac{1}{3}8) = (\frac{12}{3} - \frac{8}{3} = \frac{4}{3})$
11. $g'(x) = \frac{2x f(x) - (x^2 + 1)f'(x)}{f(x)^2}$
	$g'(2) = \frac{2(2) f(2) - (2^2 + 1)f'(2)}{f(2)^2} = \frac{2(2) (3) - (2^2 + 1)(4)}{(3)^2} = \frac{4 (3) - (4 + 1)(4)}{9} = \frac{12 - (5)(4)}{9} = \frac{12 - 20}{9} = \frac{-8}{9}$
12. $\frac{x^2 - x}{x} = x - 1$ $\int_{-1}^1 (x - 1) dx = (0.5x^2 - x)|_{-1}^1 = (0.5(1)^2 - (1)) - (0.5(-1)^2 - (-1))$
	$= (0.5(1)^2 - 1) - (0.5(-1)^2 +1) = (0.5(1) - 1) - (0.5(1) +1) = (0.5 - 1) - (0.5 +1) = (-0.5) - (1.5) = -2$
13.  MVT
14. $a(t) = 12t$
	$v(t) = 6t^2+C$
	$v(t) = 6t^2 + 2$
	$x(t) = 2t^3 + 2t + C$
	$x(t) = 2t^3 + 2t + 5$
15. $-22 = -50 + 28$
    $-2(5) = -10$
16. $\frac{dy}{dx} = 2 - y$
    $\frac{1}{2 - y}dy = dx$
    $-\ln(2 - y) = x + C$
    $-\ln(2 - 1) = 1 + C$
    $-\ln(1) = 1 + C$
    $0 = 1 + -1$
    $-e = 1 + (-1)$
    $-\ln(2 - y) = x -1$
    $\ln(2 - y) = -x + 1$
    $2 - y = e^{-x + 1}$
    $y = 2 -e^{-x + 1}$
17. $2t -  5$
---
19. $v(1) = 3 - 8 + 4 = -1$; $a(1) = 6 - 8 = -2$
---
23. $\int_0^1 (e^x)^2 dx = \int_0^1 e^{2x} dx = 0.5e^{2x}|_0^1 = 0.5e^2 - 0.5e^0 = 0.5e^2 - 0.5$
---
28. $\tan(\theta) = \frac{h}{30}$
    $\cos(\theta)/\sin(\theta) = \frac{h}{30}$
    $\frac{-\sin(\theta)\sin(\theta) - \cos(\theta)\cos(\theta)}{\sin(\theta)^2} = \frac{1}{30} = \cos(\theta)\cos(\theta) = \frac{1}{30}$
---
38. $k^3 + 3 = \frac{16}{k^2 - 3}$
    $(k^2 - 3)(k^3 + 3) = 16$
    $k^2(1 - 3)(k + 3) = 16$
    $k^2(-2)(k + 3) = 16$
    $k<0 \implies k\neq k$
---
26. $y(0) = 0$
    $y(1) = 1$
    $y'(x)=4x^{\frac{1}{3}} - 2$
    $y'(x) = 0 \implies 2 = 4x^\frac{1}{3} \implies 0.5 = \sqrt[3]{x} \implies x = 0.5^3 = 0.125$
    $y(0.125) = 3(0.125)^{4/3} - 0.25 < 0$
    