# Unit 3 - Advanced Derivatives

41. chain rule!
42. $g'(x) = 3\cos(3x)$. $g'(\pi) = 3\cos(3\pi) = -3$
43. $f'(x) = h'(x) * g'(h(x)) = 2 * g'(3) = 2 * -2 = -4$
44. $h'(x) = f'(x) * 3f(x)^2$. $h'(2) = 0.5 * 3 * 1 = \frac32$
45. $5(4x^2 - 3)^4 * (8x)$
46. $y + (-e^{3}) = -3e^{3}(x - 1)$
47. $\frac{d}{dx} [\cos(3x)^2] = 3 * -\sin(3x) * 2\cos(3x) = -6\sin(3x)\cos(3x)$
48. $\ln'(f(x)) f'(x) = \frac{f'(x)}{f(x)}$
49. $\sqrt x + y^2 = xy + 2$
	$\frac{0.5}{\sqrt x} + 2y \frac {dy}{dx} = y + \frac {dy}{dx}x$
	$\frac{0.5}{\sqrt x} - y = \frac {dy}{dx}x - 2y \frac {dy}{dx}$
	$\frac{0.5}{\sqrt x} - y = \frac {dy}{dx}(x - 2y)$
	$\frac{\frac{0.5}{\sqrt x} - y}{x - 2y}= \frac {dy}{dx}$
	$\frac{\frac{0.5}{\sqrt 4} - 0}{4 - 2*0}$
	$\frac{\frac{0.5}{\sqrt 4}}{4}$
	$\frac{0.25}{4}$
	$\frac{1}{16}$
50. $\cos(y) = x$
	$\frac{dy}{dx} * -\sin(y) = 1$
	$\frac{dy}{dx} = \frac{1}{-\sin(y)}$
	$\frac{dy}{dx} = \csc(y)$
51. $3x - xy = y^2 + 3$
	$3 - (y + \frac {dy}{dx}x) = 2y\frac {dy}{dx}$
	$3 - y - \frac {dy}{dx}x = 2y\frac {dy}{dx}$
	$3 - y = 2y\frac {dy}{dx} + \frac {dy}{dx}x$
	$3 - y = \frac {dy}{dx}(2y + x)$
	$\frac{3 - y}{2y + x} = \frac {dy}{dx}$
	$\frac{3 - 1}{2(1) + (2)} = \frac {dy}{dx}$
	$\frac{3 - 1}{2 + (2)} = \frac {dy}{dx}$
	$\frac{2}{4} = \frac {dy}{dx}$
	$\frac{1}{2} = \frac {dy}{dx}$
52. $\frac{y - \frac{dy}{dx} x}{y^2} = 1 - \frac{dy}{dx}$
	$y - \frac{dy}{dx} x = y^2 - \frac{dy}{dx}y^2$
	$y + \frac{dy}{dx}y^2 - \frac{dy}{dx} x = y^2$
	$\frac{dy}{dx}y^2 - \frac{dy}{dx} x = y^2 - y$
	$\frac{dy}{dx}(y^2 - x) = y^2 - y$
	$\frac{dy}{dx} = \frac{y^2 - y}{y^2 - x}$
53. $g'(x) = \frac 1 {f'(g(x))}$
    $g'(3) = \frac 1 {f'(g(3))}$
	$g'(3) = \frac 1 {f'(4)}$
	$g'(3) = \frac 1 {-5}$
	$g'(3) = \frac -0.2$
54. $f$ and $g$ are inverses.
   $g'(x) = \frac 1 {f'(g(x))}$ 
   $g'(x) = \frac 1 {f'(g(x))}$ 
   $g'(3) = \frac 1 {f'(g(3))}$ 
   $g'(3) = \frac 1 {f'(1)}$ 
   $g'(3) = \frac 1 {-4}$ 
   $g'(3) = -0.25$ 
55. $2\frac{1}{\tan' (\arctan(2x))}$
    $\frac{2}{\tan' (\arctan(2x))}$
	$2\cos(\arctan(2x))^2$
	$2\frac{1}{1 + (2x)^2}$
56. $\frac d {dx} \arcsin(e^x) = e^x \frac{1}{\sqrt {1 - (e^x)^2 }} = e^x \frac{1}{\sqrt {1 - e^{2x} }} = \frac{e^x}{\sqrt {1 - e^{2x} }}$
57. oh no, an implicit second derivate? 
    $2x - 2y\frac{dy}{dx} = 0$
	$-2y\frac{dy}{dx} = 2x$
	$\frac{dy}{dx} = -\frac{2x}{2y}$
	$\frac{dy}{dx} = -\frac{x}{y}$
58. üôÅ I think B logically, but I should ask how to do this mathematically.
59. Again, I suppose B?
60. $24x - 30$

# Unit 2 - Differentiation and Basic Derivative Rules

21. $\frac {f(5) - f(1)} {5 - 1} = 8$
22. $f'(-3) = 0$, $f'(0) < 0$, $f'(4) > 0$
23. $\frac d {dx} \ln(x) = \frac 1 x \implies \lim_{x\rightarrow3} \frac {\ln(x) - \ln(3)}{x-3} = \frac 1 3$
24. $\frac d {dx} \sin(x) = \cos(x)$
25. $\frac{8 - 5}{4 - 2} = \frac 3 2 = 1.5$
26. $x^{-1} + x^{-2}$
27. $x^{1.5} + 3x^{0.5}$
    $1.5x^{0.5} + 1.5x^{-0.5}$
28. continuous, but not differentiable
29. 4 (cusp)
30. $f'(x) = \cos(x) + 3\sin(x)$
	$f'(0.5\pi) = 0 + 3*1$
31. $f'(x) = \frac 1 x + 2$
    $f'(3) = \frac 1 3 + 2$
	$f'(3) = \frac 7 3$
32. $f'(x) = g(x)h'(x) + g'(x)h(x)$
    $f'(1) = (2)(4) + (-2)(3)$
	$f'(1) = 8 - 6 = 2$
33. $4x^3 e^x + e^x x^4 = e^x(x^4 + 4x^3) = e^xx^3(x + 4)$
34. $k'(x) = f'(x)h(x) + f(x)h'(x)$
    $k'(4) = (-3)(-1) + (2)(3)$
	$k'(4) = 3 + 6$
	$k'(4) = 9$
35. $f'(x) = 2\cos(x) - 2x\sin(x)$
    $f'(x) = 2\cos(x)$
	$f'(x) = 2(1)$
	$f'(x) = 2$
36. $h'(x) = \frac{g'(x)f(x) - f'(x)g(x)}{f(x)^2}$
    $h'(1) = \frac{g'(x)4 - 5g(x)}{4^2}$
	$h'(1) = \frac{3*4 - 5*2}{4^2}$
	$h'(1) = \frac{12 - 10}{16}$
	$h'(1) = \frac{2}{16}$
	$h'(1) = \frac{1}{8}$
37. $f'(x) = \frac{(6x-2)(4x+1) - (4)(3x^2 - 2x)}{(4x+1)^2}$
	$f'(x) = \frac{(6x-2)(4x+1) - 12x^2 - 8x)}{(4x+1)^2}$
	$f'(x) = \frac{(6x-2)(4x+1) - 12x^2 - 8x)}{(4x+1)^2}$
38. $f'(x) = \frac{\ln'(x) h(x) - h'(x) \ln(x)}{h(x)^2}$
    $f'(1) = \frac{\ln'(x) *-2 - -2 \ln(x)}{(-2)^2}$
	$f'(1) = \frac{\frac {-2} x + 2 \ln(1)}{(-2)^2}$
	$f'(1) = \frac{\frac {-2} x + 2 * 0}{4}$
	$f'(1) = \frac{\frac {-2} x + 0}{4}$
	$f'(1) = \frac{\frac {-2} 1}{4}$
	$f'(1) = \frac{-2}{4}$
	$f'(1) = \frac{-1}{2}$
	$f'(1) = -0.5$
39. oh boy, it's a memory one ,-,
	$-\csc(x)^2$, i think?
40. i need to study the weird trig functions more.